src/program_proof/pav/classes.v
@@ -1,0 +1,106 @@
+From Perennial.program_proof Require Import grove_prelude.
+
+Set Default Proof Using "Type*".
+
+Section classes.
+Context {PROP : bi} {A B : Type}.
+
+Class Func (f : A → B → PROP) : Prop :=
+  func x y1 y2 : f x y1 -∗ f x y2 -∗ ⌜ y1 = y2 ⌝.
+Class InjRel (f : A → B → PROP) : Prop :=
+  inj_rel x1 x2 y : f x1 y -∗ f x2 y -∗ ⌜ x1 = x2 ⌝.
+End classes.
+
+Section func_sepL.
+Context {PROP : bi} {A : Type} {Φ : nat → A → PROP}.
+
+Lemma big_sepL_func_eq l1 l2 :
+  Func Φ →
+  length l1 = length l2 →
+  ([∗ list] k↦x1 ∈ l1, Φ k x1) -∗
+  ([∗ list] k↦x1 ∈ l2, Φ k x1) -∗
+  ⌜ l1 = l2 ⌝.
+Proof.
+  revert Φ l2. induction l1 as [|x1 l1 IH]=> Φ l2 HF Hlen.
+  - destruct l2; naive_solver.
+  - destruct l2 as [|x2 l2]; [done|].
+    rewrite !big_sepL_cons.
+    iIntros "[Ha1 H1] [Ha2 H2]".
+    ospecialize (IH (λ k, Φ (S k)) l2 _ _).
+    { unfold Func in *. naive_solver. }
+    { by list_simplifier. }
+    iDestruct (IH with "H1 H2") as %->.
+    by iDestruct (HF with "Ha1 Ha2") as %->.
+Qed.
+
+Local Open Scope nat.
+
+Lemma big_sepL_func_prefix k_ub ψ l1 l2 :
+  Func Φ →
+  length l1 ≥ k_ub →
+  length l2 ≥ k_ub →
+  (∀ k, k < k_ub → Φ k = ψ k) →
+  ([∗ list] k↦x1 ∈ l1, Φ k x1) -∗
+  ([∗ list] k↦x1 ∈ l2, ψ k x1) -∗
+  ⌜ take k_ub l1 = take k_ub l2 ⌝.
+Proof.
+  iIntros (??? Heq) "H1 H2".
+  iDestruct (big_sepL_take_drop _ _ k_ub with "H1") as "[H1 _]".
+  iDestruct (big_sepL_take_drop _ _ k_ub with "H2") as "[H2 _]".
+  iDestruct (big_sepL_impl _ Φ with "H2 []") as "H2".
+  { iIntros "!>". iIntros (?? Hlook) "?".
+    rewrite Heq; [done|].
+    apply lookup_lt_Some in Hlook.
+    rewrite take_length_le in Hlook; [done|lia]. }
+  iApply (big_sepL_func_eq with "[$H1] [$H2]").
+  rewrite !take_length_le; lia.
+Qed.
+End func_sepL.
+
+Section func_sepL2.
+Context {PROP : bi} {A B : Type} {Φ : nat → A → B → PROP}.
+Context `{HF : !Func (uncurry Φ)}.
+
+Lemma big_sepL2_func_eq l1 l2 l3 :
+  ([∗ list] k↦x1;x2 ∈ l1;l2, Φ k x1 x2) -∗
+  ([∗ list] k↦x1;x2 ∈ l1;l3, Φ k x1 x2) -∗
+  ⌜ l2 = l3 ⌝.
+Proof.
+  iIntros "H1 H2".
+  iAssert (⌜ length l2 = length l3 ⌝%I) as %Hlen_eq.
+  { iDestruct (big_sepL2_length with "H1") as %?.
+    iDestruct (big_sepL2_length with "H2") as %?.
+    iPureIntro. lia. }
+  iDestruct (big_sepL2_to_sepL_2 with "H1") as "H1".
+  iDestruct (big_sepL2_to_sepL_2 with "H2") as "H2".
+  iDestruct (big_sepL_func_eq with "H1 H2") as %Heq; [|done|].
+  { iIntros (k ??) "(%a &%& H1) (% &%& H2)".
+    list_simplifier.
+    by iApply (HF (k, a) with "[H1] [H2]"). }
+  done.
+Qed.
+
+Lemma big_sepL2_func_prefix_aux l1 l2 l3 l4 :
+  l1 `prefix_of` l3 →
+  ([∗ list] k↦x1;x2 ∈ l1;l2, Φ k x1 x2) -∗
+  ([∗ list] k↦x1;x2 ∈ l3;l4, Φ k x1 x2) -∗
+  ⌜ l2 `prefix_of` l4 ⌝.
+Proof.
+  iIntros ([? ->]) "H1 H2".
+  iDestruct (big_sepL2_app_inv_l with "H2") as (??) "(%Heq & H2 &_)".
+  iDestruct (big_sepL2_func_eq with "H1 H2") as %<-.
+  list_simplifier.
+  eauto using prefix_app_r.
+Qed.
+
+Lemma big_sepL2_func_prefix l1 l2 l3 l4 :
+  l1 `prefix_of` l3 ∨ l3 `prefix_of` l1 →
+  ([∗ list] k↦x1;x2 ∈ l1;l2, Φ k x1 x2) -∗
+  ([∗ list] k↦x1;x2 ∈ l3;l4, Φ k x1 x2) -∗
+  ⌜ l2 `prefix_of` l4 ∨ l4 `prefix_of` l2 ⌝.
+Proof.
+  iIntros ([?|?]) "H1 H2".
+  - iLeft. by iApply (big_sepL2_func_prefix_aux with "H1 H2").
+  - iRight. by iApply (big_sepL2_func_prefix_aux with "H2 H1").
+Qed.
+End func_sepL2.
