src/program_proof/pav/misc.v
@@ -1,6 +1,6 @@
 From Perennial.program_proof Require Import grove_prelude.
 
-Section defs.
+Section slices.
 Context `{!heapGS Σ}.
 
 Definition is_Slice2D (sl_dim0 : Slice.t) (obj_dim0 : list (list w8)) : iProp Σ :=
@@ -33,4 +33,4 @@ Definition own_Slice3D (sl_dim0 : Slice.t) d (obj_dim0 : list (list (list w8))) 
     "#Hsep_dim1" ∷ ([∗ list] sl_dim2;obj_dim2 ∈ list_dim1;obj_dim1,
       "#Hsl_dim2" ∷ own_slice_small sl_dim2 byteT DfracDiscarded obj_dim2)).
 
-End defs.
+End slices.
