src/program_proof/pav/rpc.v
@@ -1,7 +1,7 @@
 From Perennial.program_proof Require Import grove_prelude.
 From Goose.github_com.mit_pdos.pav Require Import ktmerkle.
 
-From Perennial.program_proof.pav Require Import common.
+From Perennial.program_proof.pav Require Import misc.
 
 Module chainSepSome.
 Record t :=
